set/cunningham: 1.2. create lgical DSL to represent statements

set/cunningham/1_intro/2_Logic.v
@@ -1,91 +1,150 @@
 (** 1.2 Logical Notation *)
 Require Import Setoid.
+Require Import Morphisms.
 From Stdlib Require Import Classical.
-From Stdlib Require Import List.
-Import ListNotations.
-Open Scope bool_scope.
+From Stdlib Require Import List. Import ListNotations.
+Require Import Bool.
 Require Import Nat.
-From Stdlib Require Import NaryFunctions.
-Import SigTNotations.
+From Stdlib Require Import Strings.String.
 
-Definition bvals := [true; false].
+Open Scope bool_scope.
+
+(** Propositions and Logical Connectives *)
+(* boolean statement *)
+Inductive St :=
+| StConst (b: bool)
+| StVar (name: string)
+| StNot: St -> St
+| StAnd: St -> St -> St
+| StOr: St -> St -> St
+| StImpl: St -> St -> St
+| StIff: St -> St -> St.
+
+
+(* Notations *)
+Open Scope string_scope.
+
+Definition T: bool := true.
+Definition F: bool := false.
+Definition bvals := [F; T].
+
+Definition P: string := "P".
+Definition Q: string := "Q".
+
+(* see https://softwarefoundations.cis.upenn.edu/lf-current/Imp.html#lab403 for details *)
+Coercion StVar : string >-> St.
+Coercion StConst : bool >-> St.
+
+Declare Custom Entry st.
+Declare Scope st_scope.
+
+Notation "<{ s }>" := s (s custom st).
+Notation "( x )" := x (in custom st, x at level 99).
+Notation "x" := x (in custom st at level 0, x constr at level 0).
+Notation "x -> y" := (StImpl x y) (in custom st at level 95, right associativity).
+Notation "x <-> y" := (StIff x y) (in custom st at level 90, right associativity).
+Notation "x | y" := (StOr x y) (in custom st at level 85, right associativity).
+Notation "x & y" := (StAnd x y) (in custom st at level 80, right associativity).
+Notation "'~' b" := (StNot b) (in custom st at level 75, right associativity).
+Notation "'T'" := (StConst T) (in custom st at level 0).
+Notation "'F'" := (StConst F) (in custom st at level 0).
+Notation "'P'" := (StVar P) (in custom st at level 0).
+Notation "'Q'" := (StVar Q) (in custom st at level 0).
+
+Check <{ ~ P  -> Q }>.
+Check <{ ~(P & Q | P) <-> ~P | F }>.
+Unset Printing Notations.
+Check <{ ~(P & Q | P) <-> ~P | F }>.
+Set Printing Notations.
+
+Definition SMap (X: Type) := string -> X.
+Definition SMap_default {X: Type} (x: X): SMap X := fun _ => x.
+Definition SMap_update {X: Type} (m: SMap X) (k: string) (x: X): SMap X :=
+  fun s => if s =? k then x else m s.
+
+Notation "'_' '!->' x" := (SMap_default x) (at level 100, right associativity).
+Notation "k '!->' x ';' m" :=
+  (SMap_update m k x) (at level 100, k constr, right associativity).
+
+Definition PQ_vals: list (SMap bool) :=
+  map (fun '(p, q) => (P !-> p; Q !-> q; _ !-> F)) (list_prod bvals bvals).
+
+Fixpoint eval (m: SMap bool) (s: St): bool :=
+  match s with
+  | StConst b => b
+  | StVar name => m name
+  | StNot x => negb (eval m x)
+  | StAnd x y => (eval m x) && (eval m y)
+  | StOr x y => (eval m x) || (eval m y)
+  | StImpl x y => implb (eval m x) (eval m y)
+  | StIff x y => Bool.eqb (eval m x) (eval m y)
+  end.
+
+Fixpoint eval_prop (m: SMap Prop) (s: St): Prop :=
+  match s with
+  | StConst b => is_true b
+  | StVar name => m name
+  | StNot x => ~(eval_prop m x)
+  | StAnd x y => (eval_prop m x) /\ (eval_prop m y)
+  | StOr x y => (eval_prop m x) \/ (eval_prop m y)
+  | StImpl x y => (eval_prop m x) -> (eval_prop m y)
+  | StIff x y => (eval_prop m x) <-> (eval_prop m y)
+  end.
 
 (* Problem 1. Construct a truth table for the sentence ¬ P → (Q ∧ P) *)
-Definition pr1 (p q: bool) := implb (negb p) (q && p).
+Definition pr1 := <{ ~P -> Q & P }>.
+Compute map (fun m => (m P, m Q, eval m pr1)) PQ_vals.
 
-Compute map (fun '(p, q) => (p, q, pr1 p q)) (list_prod bvals bvals).
-(* = [(true,  true,  true);
-      (true,  false, true);
-      (false, true,  false);
-      (false, false, false)] *)
-Example pr1_is_p (p q: bool): pr1 p q = p.
-Proof. destruct p, q; reflexivity. Qed.
+Example pr1_is_p (m: SMap bool): eval m pr1 = eval m P.
+Proof. simpl. destruct (m P), (m Q); reflexivity. Qed.
 
-(* use NaryFunctions *)
-Check (bool^^3 --> bool).
-
-(* sentence *)
-Definition Snt := { n: nat & bool^^n --> bool }. (* sigT *)
-About sigT.
-About existT.
-Check (existT (fun n => bool^^n --> bool)).
-Check (existT (fun n => bool^^n --> bool) 2 andb) : Snt.
-Check (existT _ 2 andb) : Snt.
-
-Definition mkSnt (n: nat) (f: bool^^n --> bool): Snt := existT _ n f.
-Check mkSnt 2 andb.
-
-Notation "s .n" := (projT1 s) (at level 1, left associativity, format "s .n").
-Compute (mkSnt 2 andb).n.
-
-Notation "s .f" := (projT2 s) (at level 1, left associativity, format "s .f").
-Compute (mkSnt 2 andb).f.
-
-(* uncurry sentence function *)
-Definition Snt_unc (s: Snt): bool^s.n -> bool := nuncurry bool bool s.n s.f.
-
-Definition ConstB (b: bool) (s: Snt): Prop := forall x: bool^s.n, Snt_unc s x = b.
+Definition ConstB (b: bool) (s: St): Prop := forall m, eval m s = b.
 
 (** Definition 1.2.1. *)
 Definition TautologyB := ConstB true.
 
-Theorem LEMB: TautologyB (mkSnt 1 (fun p => p || negb p)).
-Proof.
-  unfold TautologyB, ConstB. destruct x. simpl.
-  destruct b; reflexivity.
-Qed.
+Definition TautologyP (s: St) := forall m, eval_prop m s.
+
+Theorem LEMB: TautologyB <{ P | ~P }>.
+Proof. intros m. simpl. destruct (m P); reflexivity. Qed.
+
+Example LEMP: TautologyP <{ P | ~P }>.
+Proof. intros m. simpl. destruct (classic (m P)); auto. Qed.
 
 (** Definition 1.2.2. *)
 Definition ContradictionB := ConstB false.
 
-Example ContradictionB__ex: ContradictionB (mkSnt 1 (fun p => p && negb p)).
+Definition ContradictionP (s: St) := forall m, ~ eval_prop m s.
+
+Example ContradictionB__ex: ContradictionB <{ P & ~P }>.
+Proof. intros m. simpl. destruct (m P); reflexivity. Qed.
+
+Example ContradictionP__ex: ContradictionP <{ P & ~P }>.
 Proof.
-  unfold ContradictionB, ConstB. destruct x. simpl.
-  destruct b; reflexivity.
+  intros m. simpl. remember (m P) as H eqn:eq. intuition.
 Qed.
 
 (** LogicalEquivalence *)
 
 (** Definition 1.2.3.
-    [P(X)] and [Q(X)] are logically equivalent (P <=> Q) iff [forall X: bool^n, P X = Q X] *)
-Definition EqB (n: nat) (f g: bool^^n --> bool) := forall x: bool^n, nuncurry _ _ n f x = nuncurry _ _ n g x.
+    [P(X)] and [Q(X)] are logically equivalent (P <=> Q) iff [forall X, P X = Q X] *)
+Definition EqB (p q: St) := forall m, eval m p = eval m q.
+Notation "p '<=>' q" := (EqB p q) (at level 70, no associativity).
 
-(* useless but interesting try to implement ideas from https://www.cis.upenn.edu/~plclub/blog/2020-05-15-Rewriting-in-Coq/ *)
-Section Useless_EqB_props.
-
-Instance EqB_refl (n: nat): Reflexive (EqB n).
+(* implement ideas from https://www.cis.upenn.edu/~plclub/blog/2020-05-15-Rewriting-in-Coq/ *)
+Instance EqB_refl: Reflexive EqB.
 Proof. unfold Reflexive, EqB. reflexivity. Qed.
 
-Instance EqB_sym (n: nat): Symmetric (EqB n).
+Instance EqB_sym: Symmetric EqB.
 Proof. unfold Symmetric, EqB. auto. Qed.
 
-Instance EqB_trans (n: nat): Transitive (EqB n).
+Instance EqB_trans: Transitive EqB.
 Proof.
   unfold Transitive, EqB.
-  intros f g h H1 H2 x. rewrite H1, H2. reflexivity.
+  intros p q r H1 H2 m. rewrite H1, H2. reflexivity.
 Qed.
 
-Instance EqB_equiv (n: nat): Equivalence (EqB n).
+Instance EqB_equiv: Equivalence EqB.
 Proof.
   split. 
   - apply EqB_refl.
@@ -93,28 +152,44 @@ Proof.
   - apply EqB_trans.
 Qed.
 
-Require Import Morphisms.
-Instance EqB_negb_proper (n: nat): Proper (EqB n ==> EqB n) (nfun_to_nfun _ _ _ negb n).
+Instance EqB_not_proper: Proper (EqB ==> EqB) StNot.
 Proof.
   unfold Proper, respectful, EqB.
-  induction n as [| n IH].
-  { simpl. intros p q H _. rewrite H.
-    - reflexivity.
-    - exact tt. }
-  intros p q eq [b x]. simpl. apply (IH (p b) (q b)). clear IH x.
-  simpl in eq. intro x. apply (eq (b, x)).
+  intros p q H m. simpl. rewrite H. reflexivity.
 Qed.
 
-End Useless_EqB_props.
+Example StNot_rewrite_ex (p q: St): p <=> q -> <{ ~p }> <=> <{ ~q }>.
+Proof. intro H. rewrite H. reflexivity. Qed.
+
+Instance EqB_and_proper: Proper (EqB ==> EqB ==> EqB) StAnd.
+Proof.
+  unfold Proper, respectful, EqB.
+  intros p1 q1 H1 p2 q2 H2 m. simpl. rewrite H1, H2. reflexivity.
+Qed.
+
+Instance EqB_or_proper: Proper (EqB ==> EqB ==> EqB) StOr.
+Proof.
+  unfold Proper, respectful, EqB.
+  intros p1 q1 H1 p2 q2 H2 m. simpl. rewrite H1, H2. reflexivity.
+Qed.
+
+Instance EqB_impl_proper: Proper (EqB ==> EqB ==> EqB) StImpl.
+Proof.
+  unfold Proper, respectful, EqB.
+  intros p1 q1 H1 p2 q2 H2 m. simpl. rewrite H1, H2. reflexivity.
+Qed.
+
+Instance EqB_iff_proper: Proper (EqB ==> EqB ==> EqB) StIff.
+Proof.
+  unfold Proper, respectful, EqB.
+  intros p1 q1 H1 p2 q2 H2 m. simpl. rewrite H1, H2. reflexivity.
+Qed.
 
 (* De Morgan’s Laws *)
-Theorem DMLB1 (p q: bool): negb (p || q) = negb p && negb q.
-Proof. destruct p, q; reflexivity. Qed.
-
-Theorem DMLB1': EqB 2 (fun p q => negb (p || q)) (fun p q => negb p && negb q).
+Theorem DMLB1 (p q: St): <{ ~(p | q) }> <=> <{ ~p & ~q }>.
 Proof.
-  unfold EqB. intros [p [q z]]. simpl. clear z.
-  destruct p, q; reflexivity.
+  unfold EqB. intro m. simpl.
+  destruct (eval m p), (eval m q); reflexivity.
 Qed.
 
 Theorem DML1 (P Q: Prop): ~(P \/ Q) <-> ~P /\ ~Q.
@@ -126,8 +201,11 @@ Proof.
   - destruct H as [HnP HnQ]. intros [C | C]; auto.
 Qed.
 
-Theorem DMLB2 (p q: bool): negb (p && q) = negb p || negb q.
-Proof. destruct p, q; reflexivity. Qed.
+Theorem DMLB2 (p q: St): <{ ~(p & q) }> <=> <{ ~p | ~q }>.
+Proof.
+  unfold EqB. intro m. simpl.
+  destruct (eval m p), (eval m q); reflexivity.
+Qed.
 
 Theorem DML2 (P Q: Prop): ~(P /\ Q) <-> ~P \/ ~Q.
 Proof.
@@ -137,3 +215,6 @@ Proof.
     + left. exact HnP.
   - intros [HP HQ]. destruct H; contradiction.
 Qed.
+
+Example apply_DML2: <{ ~((P -> Q) & (Q -> P)) }> <=> <{ ~(P -> Q) | ~(Q -> P) }>.
+Proof. rewrite DMLB2. reflexivity. Qed.
